proved refinement

proof/Refinement.v
@@ -11,12 +11,162 @@ From Scheduler.PartitionMockup Require  Import Primitives.
 From Scheduler Require  Import EDF.
 
 
+Module FunctionalEdfWithFuelMod(J : JobsAxiomsMod).
+Import J.
+
+  
+Module F:= FunctionalEdfImplementsAssumptionsMod J.
+Import F.
+
+Module S :=  FunctionalEdfIsCorrectMod J.
+Import S.
+
+Fixpoint functional_insert_new_entries_fuel(timeout : nat) (new_jobs : list nat)(active : list Entry) : list Entry :=
+  match timeout with
+    0 => active
+  | S timeout1  =>
+    match new_jobs with
+      [] => active
+    |  new_job_id :: remaining_jobs =>
+      
+      let new_entry :=  mk_Entry
+            new_job_id
+            (budget (Jobs new_job_id))
+            (S (deadline (Jobs new_job_id) - (arrival (Jobs new_job_id)))) in
+      let active1 := insert _
+         (fun e1 e2 : Entry =>
+            deadline (Jobs (id e1)) <=? deadline (Jobs (id e2)))
+         new_entry active in
+      functional_insert_new_entries_fuel timeout1 remaining_jobs active1
+    end
+  end.
+
+Lemma functional_insert_new_entries_enough_fuel :
+  forall  l n  l' ,
+    length l <= n ->
+    functional_insert_new_entries_fuel n  l l'  =
+    insert_all _
+               (fun e1 e2 : Entry =>
+                                         deadline (Jobs (id e1)) <=? deadline (Jobs (id e2)))
+            (map
+             (fun j  =>
+             {|
+             id :=  j;
+             cnt := budget (Jobs j);
+             del := S (deadline (Jobs j) - (arrival (Jobs j))) |}) l)
+            l'.
+Proof.
+induction l ; intros n l' Hlen.
+*   cbn.
+    destruct n ; auto.
+*  cbn.
+   cbn in Hlen.
+   destruct n ; try lia.
+   rewrite <- IHl with ( n:= n) ; auto ; try lia.
+Qed.
+
+Definition functional_update_entries_fuel(s:State) : ((option nat *bool)* State) :=
+  let  l :=
+     filter (fun j =>  j <? N) (jobs_arriving_at s.(now))  in                                     
+let b := 
+     match hd_error s.(active) with
+     | Some e =>
+         let j := Jobs (id e) in
+         (cnt e <=? budget j - duration j)
+     | None => false
+     end
+in
+let b' :=  match hd_error s.(active) with
+     | Some e =>
+         cnt e =? 0
+     | None => false
+           end
+in
+let b'' :=  match hd_error s.(active) with
+     | Some e =>
+         del e =? 0
+     | None => false
+           end
+in             
+let active1 := if b && (negb b') then tl s.(active) else s.(active) in
+let active2 :=
+       functional_insert_new_entries_fuel N  l  active1  in
+
+( match active2 with
+     | [] => (None,b'')
+     | e :: _ => (Some (id e), b'')
+  end,  mk_State  s.(now) active2).
+
+
+Lemma  functional_update_entries_enough_fuel : forall s, 
+  functional_update_entries s = functional_update_entries_fuel s.
+Proof.
+intros s.
+unfold functional_update_entries, functional_update_entries_fuel.
+rewrite functional_insert_new_entries_enough_fuel; auto.
+apply pigeon_hole.
+*  apply NoDup_filter.
+   rewrite NoDup_nth.
+   intros i j Hi Hj Heq.
+   destruct (jobs_arriving_at_unique _ _ _ _ Hi Hj Heq); auto.
+* intros i Hin.
+  rewrite filter_In in Hin.
+  destruct Hin as (_ & Hlt).
+  rewrite NPeano.Nat.ltb_lt in Hlt ; auto.
+Qed.
+
+
+Definition functional_scheduler_fuel  (s: State)  :=
+  let (r,s')  := functional_update_entries_fuel  s in
+  let (_,s'') := functional_update_counters  s' in
+  (r,s'').                
+
+Lemma functional_scheduler_enough_fuel  : forall s,
+    functional_scheduler_fuel s = functional_scheduler s.
+Proof.
+intros s.
+unfold functional_scheduler, functional_scheduler_fuel.
+rewrite functional_update_entries_enough_fuel ; auto.
+Qed.
+
+Fixpoint functional_scheduler_star_fuel (t: nat):=
+  match t with
+    0 => ((None,false),init)
+  |S t' =>
+   let (_,s') := functional_scheduler_star_fuel  t' in
+   functional_scheduler_fuel  s'
+  end.
+
+
+Lemma functional_scheduler_star_fuel_S : forall  t,
+    functional_scheduler_star_fuel (S t) =
+     let (_,s') := functional_scheduler_star_fuel t in
+     functional_scheduler_fuel s'.
+Proof.
+reflexivity.
+Qed.
+
+Lemma functional_scheduler_star_enough_fuel : forall t,
+     functional_scheduler_star_fuel t =  functional_scheduler_star t.
+Proof.
+induction t ; auto.
+rewrite functional_scheduler_star_S,functional_scheduler_star_fuel_S.
+rewrite IHt.
+remember (functional_scheduler_star t) as rs ; destruct rs as (r,s).
+unfold functional_scheduler_fuel, Alg.functional_scheduler.
+rewrite functional_update_entries_enough_fuel ; auto.
+Qed.
+
+End FunctionalEdfWithFuelMod.
+
 Module RefinementMod (J :JobsAxiomsMod).
  Import J.
   
 Module F:= FunctionalEdfImplementsAssumptionsMod J.
 Import F. 
 
+Module FF := FunctionalEdfWithFuelMod J.
+Import FF.
 
 Definition E :  Env := (fun k =>
                            (map (fun j =>
@@ -45,9 +195,7 @@ Definition update_first_entry (finished expired : CBool) :=
   else
     ret tt).
 
-Definition add_new_entries (new_jobs : JobSet) :=  
-  do new_jobs_length <- get_length new_jobs ;
-  insert_new_entries new_jobs new_jobs_length.
+
 
 Definition write_output (late : CBool) :=
   do no_active_entry <- is_active_list_empty;
@@ -70,7 +218,7 @@ Definition decomposed_update_entries :=
   do tuple <- read_inputs;
   match tuple with (new_jobs, finished,expired,late) =>
     update_first_entry finished expired ;;
-    add_new_entries new_jobs ;;
+    insert_new_entries new_jobs ;;
     write_output late
   end.
  
@@ -78,7 +226,7 @@ Definition decomposed_update_entries :=
 Lemma decomposition_correct :
      update_entries = decomposed_update_entries .
 Proof.
- unfold decomposed_update_entries, update_entries, read_inputs, update_first_entry, add_new_entries, write_output in *.
+ unfold decomposed_update_entries, update_entries, read_inputs, update_first_entry, insert_new_entries, write_output in *.
  rewrite bind_bind.
  f_equal.
  extensionality new_jobs.
@@ -121,18 +269,13 @@ Definition functional_update_first_entry (s : State) (b b' : bool) :=
   let active1 := if b && (negb b') then tl s.(active) else s.(active) in
   (tt,mk_State s.(now) active1).
 
-Definition functional_add_new_entries(s:State) (l : list nat) :=
+Definition functional_add_new_entries_fuel(s:State) (l : list nat) :=
  let active2 :=
-       insert_all _
-         (fun e1 e2 : Entry =>
-          deadline (Jobs (id e1)) <=? deadline (Jobs (id e2)))
-         (map
-            (fun j  =>
-             {|
-             id :=  j;
-             cnt := budget (Jobs j);
-             del := S (deadline (Jobs j) - (arrival (Jobs j))) |}) l) s.(active) in
+       functional_insert_new_entries_fuel  N l s.(active) in
  (tt,mk_State s.(now) active2).
+
+
+
 
 
 Definition functional_write_output (s : State) (b'' : bool) :=
@@ -145,20 +288,20 @@ Definition functional_decomposed_update_entries(s : State) :=
   let (tuple,s') :=  functional_read_inputs s in
   match tuple with (l, b,b',b'') =>
     let (_,s'') := functional_update_first_entry  s' b b' in
-    let (_,s''') := functional_add_new_entries s'' l in
+    let (_,s''') := functional_add_new_entries_fuel s'' l in
     functional_write_output s''' b'' 
   end.
 
 
 Lemma functional_decomposition_correct :
-     functional_update_entries = functional_decomposed_update_entries .
+     functional_update_entries_fuel = functional_decomposed_update_entries .
 Proof.
   auto.
 Qed.
 
 
 
-Lemma functional_read_inputs_refines_monadic :  forall r s0 s,
+Lemma read_inputs_refinement :  forall r s0 s,
     read_inputs E s0 = (r,s) ->  functional_read_inputs s0 = (r,s).
 Proof.
 intros r s0 s Hr.
@@ -217,7 +360,7 @@ Qed.
 
 
 
-Lemma functional_update_first_entry_refines_monadic :  forall b b' r s0 s,
+Lemma update_first_entry_refinement :  forall b b' r s0 s,
     update_first_entry b b' E s0 = (r,s) ->
     functional_update_first_entry s0 b b'  = (r,s).
 Proof.  
@@ -233,14 +376,114 @@ destruct s.
 f_equal ; auto.
 Qed.
 
-Lemma functional_add_new_entries_refines_monadic :  forall l r s0 s,
-    add_new_entries l E s0 = (r,s) ->
-    functional_add_new_entries s0 l  = (r,s).
-Proof.  
-Admitted.
+
+Lemma insert_new_entries_now :   forall l r s0 s,
+    insert_new_entries_aux N  l  E s0 = (r,s) -> now s0 = now s.
+Proof.
+  induction N ; intros l r s0 s Hins.  
+  * cbn in Hins.
+    injection Hins ; intros  ; subst ; auto.
+  *  cbn in Hins.
+     destruct l.
+  +
+    injection Hins ; intros ; subst; auto.
+  + 
+     unfold get_first_job_id,  get_remaining_jobs, create_entry_from_job_id, get_job_from_job_id,
+    get_budget, get_deadline, get_arrival, make_entry, sub, succ,
+    cmp_entry_deadline,insert_new_active_entry,ret,bind in Hins.
+    cbn [tl] in Hins.    
+    remember  {|
+           now := now s0;
+           active := insert_Entry_aux
+                       {|
+                       id := c1;
+                       cnt := budget (Jobs c1);
+                       del := S
+                                (deadline (Jobs c1) -
+                                 arrival (Jobs c1)) |}
+                       (active s0)
+                       (fun entry1 entry2 : Entry =>
+                        deadline (Jobs (id entry1)) <=?
+                        deadline (Jobs (id entry2))) |} as s1.
+    rewrite <-  (IHc0  _ _ _ _  Hins), Heqs1 ; auto.    
+Qed.
+
+Lemma insert_entry_active : forall e l,
+   insert_Entry_aux
+    e
+    l
+    (fun entry1 entry2 : Entry =>
+     deadline (Jobs (id entry1)) <=? deadline (Jobs (id entry2))) =
+  insert Entry
+    (fun e1 e2 : Entry =>
+     deadline (Jobs (id e1)) <=? deadline (Jobs (id e2)))
+    e
+    l.
+Proof.
+induction l ; auto.
+cbn.
+case (deadline (Jobs (id e)) <=? deadline (Jobs (id a))) ; auto.
+rewrite IHl ; auto.
+Qed.
+
+Lemma insert_new_entries_active :   forall l r s0 s,
+    insert_new_entries_aux N  l E s0 = (r,s) ->
+    active s = functional_insert_new_entries_fuel N l
+    (active s0).
+Proof.
+  induction N; intros l r s0 s Hins.
+* cbn in *.
+  injection Hins ; intros ; subst;auto.
+* cbn in Hins.
+  destruct l.
+  +  
+        injection Hins ; intros ; subst ; auto.
+  +
+    
+    unfold get_first_job_id,  get_remaining_jobs, create_entry_from_job_id, get_job_from_job_id,
+    get_budget, get_deadline, get_arrival, make_entry, sub, succ,
+    cmp_entry_deadline,insert_new_active_entry,ret,bind in Hins.
+    cbn [tl] in Hins.
+    remember  {|
+           now := now s0;
+           active := insert_Entry_aux
+                       {|
+                       id := c1;
+                       cnt := budget (Jobs c1);
+                       del := S
+                                (deadline (Jobs c1) -
+                                 arrival (Jobs c1)) |}
+                       (active s0)
+                       (fun entry1 entry2 : Entry =>
+                        deadline (Jobs (id entry1)) <=?
+                        deadline (Jobs (id entry2))) |} as s1.
+    rewrite (IHc0  _ _ _ _  Hins).
+    cbn.
+    f_equal ; auto.
+    rewrite Heqs1.
+    cbn.
+    apply insert_entry_active.
+Qed.
+    
+Lemma add_new_entries_refinement :  forall l r s0 s,
+    insert_new_entries l E s0 = (r,s) ->
+    functional_add_new_entries_fuel s0 l  = (r,s).
+Proof.
+intros l r s0 s Ha.
+destruct r.  
+unfold functional_add_new_entries_fuel.
+f_equal.
+unfold insert_new_entries,
+bind,ret in Ha.
+replace s with {| now := s.(now) ; active := s.(active) |} ; [ | destruct s ; auto].
+f_equal.
+* eapply insert_new_entries_now; eauto.
+* symmetry.
+  erewrite insert_new_entries_active ; eauto.
+Qed.
 
 
-Lemma functional_write_output_refines_monadic :  forall b'' r s0 s,
+Lemma write_output_refinement :  forall b'' r s0 s,
     write_output b'' E s0 = (r,s) ->
     functional_write_output s0 b''  = (r,s).
 Proof.
@@ -259,8 +502,8 @@ destruct as0.
   destruct s ; f_equal ; auto.
 Qed.
 
-Lemma functional_update_entries_refines_monadic :  forall r s0 s,
-   update_entries E s0 = (r,s) ->  functional_update_entries s0 = (r,s).
+Lemma update_entries_refinement :  forall r s0 s,
+   update_entries E s0 = (r,s) ->  functional_update_entries_fuel s0 = (r,s).
 Proof.
 intros r s0 s Hu.  
 rewrite decomposition_correct in Hu.
@@ -275,7 +518,7 @@ remember (read_inputs E s0) as ri.
 destruct ri as (r',s').
 symmetry in Heqri.
 generalize Heqri  ; intro Heqri_cp.
-rewrite <- functional_read_inputs_refines_monadic with (s0 := s0) in Heqri ; auto.
+rewrite <- read_inputs_refinement with (s0 := s0) in Heqri ; auto.
 assert (Heq  : (r,s) = (r',s') ) ; [congruence | ].
 injection Heq ; intros ; subst.
 clear s0 Heq Heqri Heqri_cp Heqfri.
@@ -286,18 +529,18 @@ remember (update_first_entry b b' E s') as ri.
 destruct ri as (r'',s'').
 symmetry in Heqri.
 generalize Heqri  ; intro Heqri_cp.
-erewrite <- functional_update_first_entry_refines_monadic with (s0 := s') in Heqri ; eauto.
+erewrite <- update_first_entry_refinement with (s0 := s') in Heqri ; eauto.
 assert (Heq  : (r,s) = (r'',s'') ) ; [congruence | ].
 injection Heq ; intros ; subst.
 clear s' Heq Heqri Heqri_cp Heqfri r''.
 
-remember (functional_add_new_entries s'' l) as fri.
+remember (functional_add_new_entries_fuel s'' l) as fri.
 destruct fri as (r,s).
-remember (add_new_entries l E s'') as ri.
+remember (insert_new_entries l E s'') as ri.
 destruct ri as (r',s').
 symmetry in Heqri.
 generalize Heqri  ; intro Heqri_cp.
-erewrite <- functional_add_new_entries_refines_monadic with (s0 := s'') in Heqri ; eauto.
+erewrite <- add_new_entries_refinement with (s0 := s'') in Heqri ; eauto.
 assert (Heq  : (r,s) = (r',s') ) ; [congruence | ].
 injection Heq ; intros ; subst.
 clear  Heq Heqri Heqri_cp Heqfri r' s'' b b' l.
@@ -305,11 +548,11 @@ clear  Heq Heqri Heqri_cp Heqfri r' s'' b b' l.
 
 remember (write_output b'' E s') as ri.
 destruct ri as (r'',s'').
-erewrite functional_write_output_refines_monadic; eauto.
+erewrite write_output_refinement; eauto.
 Qed.
 
 
-Lemma functional_update_counters_refines_monadic :  forall r s0 s,
+Lemma update_counters_refinement :  forall r s0 s,
    update_counters E s0 = (r,s) ->  functional_update_counters s0 = (r,s).
 Proof.
 unfold update_counters, functional_update_counters.
@@ -392,14 +635,14 @@ cbn in *.
 Qed.
 
 
-Lemma functional_edf_refines_monadic :  forall r s0 s,
-   scheduler E s0 = (r,s) ->  functional_scheduler s0 = (r,s).
+Lemma edf_refinement_fuel :  forall r s0 s,
+   scheduler E s0 = (r,s) ->  functional_scheduler_fuel s0 = (r,s).
 Proof.
-unfold scheduler, functional_scheduler.  
+unfold scheduler, functional_scheduler_fuel.  
 intros r s0 s Hs.
-remember (functional_update_entries s0) as fe.
+remember (functional_update_entries_fuel s0) as fe.
 destruct fe as (r0,s').
-remember  (functional_update_counters s') as fc.
+remember  (F.functional_update_counters s') as fc.
 destruct fc.
 unfold bind, ret in Hs.
 remember (update_entries E s0) as as'.
@@ -407,13 +650,22 @@ destruct as' as (a',s'').
 remember (update_counters E s'') as as'.
 destruct as'.
 injection Hs ; intros ; subst ; clear Hs.
-rewrite functional_update_entries_refines_monadic
+rewrite update_entries_refinement
   with (r := r) (s := s'')in Heqfe ; [ | rewrite Heqas'; reflexivity].
 injection Heqfe ; intros ; subst. 
-rewrite  functional_update_counters_refines_monadic
+rewrite  update_counters_refinement
   with (r := u0)(s := s) in Heqfc ; [ | rewrite Heqas'0; reflexivity].
 injection Heqfc; intros; subst.
 reflexivity.
+Qed.
+
+
+Lemma edf_refinement :  forall r s0 s,
+   scheduler E s0 = (r,s) ->  functional_scheduler s0 = (r,s).
+Proof.
+ intros r s0 s Hs.
+apply edf_refinement_fuel in Hs.  
+rewrite <- functional_scheduler_enough_fuel ; auto. 
 Qed.
 
 End RefinementMod.
